src/Analysis/Equations/Constraint_System.thy
@@ -641,4 +641,5 @@ locale sound_effectful_transfer =
     "\<forall>cc ex \<sigma>. \<forall>s \<in> \<lbrakk>\<sigma> (Inl cc) \<squnion> glob_env \<sigma>\<rbrakk>.
        \<forall>t \<in> \<lbrakk>\<sigma> (Inl ex) \<squnion> glob_env \<sigma>\<rbrakk>.
          <s|t> \<in> \<lbrakk>etf_full (etf_combine etf cc ex) \<sigma>\<rbrakk>"
+
 end
